Generalised fair sched example further

theories/examples/fair_sched.v
@@ -2,42 +2,43 @@ From ltl Require Import ltl ltl_fixpoints ltl_now classical ltl_adequacy.
 
 Import tProp.
 
-
 Section fair_sched.
+  Context (state : Set).
+  Context (next : state → state).
+  Context (f : state → nat).
   Context (label : Set).
-  Context (f : nat → label).
-
-  Notation state := nat.
+  Context (g : state → label).
+  Context (Hg : ∀ s i, f s = i → f (next s) = S i).
 
   Inductive steps : state → label → state → Prop :=
-  | my_step_succ i : steps i (f i) (i+1)
-  | my_step_fail i j : f i ≠ j → steps i j i.
+  | my_step_succ s : steps s (g s) (next s)
+  | my_step_fail s j : g s ≠ j → steps s j s.
 
   Notation tProp := (tProp state label steps).
 
   Axiom advanced_fair : ∀ i, ⊢ ◊ ↓l i : tProp.
 
-  Lemma step i :
-    ↓s i ⊢ ∃ l, ↓l l ∧
-                ((⌜f i = l⌝ ∧ ○ ↓s (i+1)) ∨
-                (⌜f i ≠ l⌝ ∧ ○ (↓s i))) : tProp.
+  Lemma step (s:state) :
+    ↓s s ⊢ ∃ (l:label), ↓l l ∧
+                ((⌜g s = l⌝ ∧ ○ ↓s (next s)) ∨
+                 (⌜g s ≠ l⌝ ∧ ○ (↓s s))) : tProp.
   Proof.
     iIntros "H".
     iDestruct (trace_steps with "H") as (l s' Hsteps') "[Hl Hs]";
       [by eexists _, _; constructor|].
     inversion Hsteps'; simplify_eq.
-    - iExists (f i). iFrame. iLeft. iFrame. done. 
+    - iExists (g s). iFrame. iLeft. iFrame. done. 
     - iExists l. iFrame. iRight. iFrame. done.
   Qed.
 
-  Lemma eventually_incr i :
-    ↓s i ⊢ ◊ ↓s (i+1) : tProp.
+  Lemma eventually_incr s :
+    ↓s s ⊢ ◊ ↓s (next s) : tProp.
   Proof.
     iIntros "Hs".
-    iAssert (↓s i ∪ ↓s (i+1))%I with "[Hs]" as "H"; last first.
+    iAssert (↓s s ∪ ↓s (next s))%I with "[Hs]" as "H"; last first.
     { by iApply (ltl_until_mono_strong with "[] [] H"); eauto. }
     iRevert "Hs".
-    iDestruct (advanced_fair (f i)) as "-#Hfair".
+    iDestruct (advanced_fair (g s)) as "-#Hfair".
     iApply (ltl_eventually_ind_strong with "[] Hfair").
     iIntros "!> [Hl|H]".
     { iIntros "Hs".
@@ -58,7 +59,7 @@ Section fair_sched.
   Qed.
 
   Lemma eventually_n n :
-    ↓s 0 ⊢ ◊ ↓s n : tProp.
+    ↓fs f 0 ⊢ ◊ ↓fs f n : tProp.
   Proof.
     assert (∃ i j, i = 0 ∧ n-j = i ∧ n >= j) as (i&j&<-&H1&H2).
     { eexists _, n. split; [done|]. lia. }
@@ -66,41 +67,74 @@ Section fair_sched.
     { simplify_eq. rewrite right_id. iIntros "H".
       by iApply ltl_eventually_intro_now. }
     iIntros "Hi".
-    iDestruct (eventually_incr with "Hi") as "H'".
+    iDestruct (ltl_now_state_f_frame with "Hi") as (s Hs) "Hs".
+    iDestruct (eventually_incr with "Hs") as "H'".
     iApply (ltl_eventually_ind_strong with "[] H'").
     iIntros "!> [H|(H3&H2)]".
     { iApply "IHj".
       { instantiate (1:=i+1). rewrite -H1. iPureIntro. lia. }
       { iPureIntro. lia. }
-      iFrame. }
+      iApply ltl_now_state_f_frame. iExists _.
+      iFrame. 
+      iPureIntro. erewrite Hg; [|done]. lia. }
     by iApply ltl_next_eventually.
   Qed.
 
 End fair_sched.
 
-Section fair_coin.
+Module incr.
+
+  Definition state : Set := nat.
+  Definition label : Set := ().
+  Definition f (_:state) := ().
+  Definition g : nat → nat := id.
+  Definition next := S.
+
+  Notation tProp := (tProp state label (steps state next label f)).
+
+  Lemma eventually_n_coin n :
+    ↓s 0 ⊢ ◊ ↓s n : tProp.
+  Proof.
+    apply eventually_n. 
+    naive_solver.
+  Qed.
+  
+End incr.
+
+Module fair_coin.
 
   Definition state : Set := nat.
   Definition label : Set := bool.
   Definition f := Nat.even.
+  Definition g : nat → nat := id.
+  Definition next := S.
 
-  Notation tProp := (tProp state label (steps label f)).
+  Notation tProp := (tProp state label (steps state next label f)).
 
   Lemma eventually_n_coin n :
     ↓s 0 ⊢ ◊ ↓s n : tProp.
-  Proof. apply eventually_n. Qed.
+  Proof.
+    apply eventually_n. 
+    naive_solver.
+  Qed.
 
 End fair_coin.
 
-Section fair_inf.
+Module fair_inf.
 
-  Definition inf_state : Set := nat.
-  Definition inf_label : Set := nat.
+  Definition state : Set := nat.
+  Definition label : Set := nat.
+  Definition f : state → label := id.
+  Definition g : state → state := id.
+  Definition next := S.
 
-  Notation tProp := (tProp state inf_label (steps inf_label id)).
+  Notation tProp := (tProp state label (steps state next label f)).
 
   Lemma eventually_n_inf n :
     ↓s 0 ⊢ ◊ ↓s n : tProp.
-  Proof. apply eventually_n. Qed.
+  Proof.
+    apply eventually_n. 
+    naive_solver.
+  Qed.
 
 End fair_inf.
